Annotate with explicit types

DListRef.fst
@@ -26,22 +26,25 @@ type dlisthead (t:Type0) ={
 }
 
 (** Initialize an element of a doubly linked list *)
-let empty_entry (#t:Type) (payload:t) : dlist t =
+val empty_entry: #t:Type -> payload:t -> dlist t
+let empty_entry #t payload =
   { flink = None ; blink = None ; p = payload }
 
 (** Initialize a doubly linked list head *)
-let empty_list (#t:Type) : dlisthead t =
+val empty_list: #t:Type -> dlisthead t
+let empty_list #t =
   { lhead = None ; ltail = None ; nodes = hide createEmpty }
 
-let getSome (a : option 't{isSome a}) =
-  Some?.v a
+val getSome: (a:option 'a{isSome a}) -> (b:'a{a == Some b})
+let getSome a = Some?.v a
 
-let (@) (a:ref 't) (h0:heap) = sel h0 a
-let (^@) (a:option (ref 't){isSome a}) (h0:heap) = (getSome a) @ h0
+unfold let (@) (a:ref 't) (h0:heap) = sel h0 a
+unfold let (^@) (a:option (ref 't){isSome a}) (h0:heap) = (getSome a) @ h0
 
-let (.[]) (s:seq 'a) (n:nat{n < length s}) = index s n
+unfold let (.[]) (s:seq 'a) (n:nat{n < length s}) = index s n
 
-let flink_valid (#t:Type) (h0:heap) (h:dlisthead t) =
+val flink_valid: #t:Type -> h0:heap -> h:dlisthead t -> Type0
+let flink_valid #t h0 h =
   let nodes = reveal h.nodes in
   let len = length nodes in
   (forall i. {:pattern (nodes.[i]).flink}
@@ -49,7 +52,8 @@ let flink_valid (#t:Type) (h0:heap) (h:dlisthead t) =
       isSome (nodes.[i]).flink /\
       (nodes.[i]).flink^@h0 == nodes.[i+1]))
 
-let blink_valid (#t:Type) (h0:heap) (h:dlisthead t) =
+val blink_valid: #t:Type -> h0:heap -> h:dlisthead t -> Type0
+let blink_valid #t h0 h =
   let nodes = reveal h.nodes in
   let len = length nodes in
   (forall i. {:pattern (nodes.[i]).blink}
@@ -57,7 +61,8 @@ let blink_valid (#t:Type) (h0:heap) (h:dlisthead t) =
       isSome (nodes.[i]).blink /\
       (nodes.[i]).blink^@h0 == nodes.[i-1]))
 
-let dlisthead_ghostly_connections (#t:Type) (h0:heap) (h:dlisthead t) =
+val dlisthead_ghostly_connections: #t:Type -> h0:heap -> h:dlisthead t -> Type0
+let dlisthead_ghostly_connections #t h0 h =
   let nodes = reveal h.nodes in
   let len = length nodes in
   let empty = (len = 0) in
@@ -68,7 +73,8 @@ let dlisthead_ghostly_connections (#t:Type) (h0:heap) (h:dlisthead t) =
     h.lhead^@h0 == nodes.[0] /\
     h.ltail^@h0 == nodes.[len-1])
 
-let dlisthead_is_valid (#t:Type) (h0:heap) (h:dlisthead t) =
+val dlisthead_is_valid: #t:Type -> h0:heap -> h:dlisthead t -> Type0
+let dlisthead_is_valid #t h0 h =
   let nodes = reveal h.nodes in
   let len = length nodes in
   let empty = (len = 0) in
@@ -77,29 +83,34 @@ let dlisthead_is_valid (#t:Type) (h0:heap) (h:dlisthead t) =
               flink_valid h0 h /\
               blink_valid h0 h)
 
-let test1 () = assert (forall h0 t. dlisthead_is_valid h0 (empty_list #t))
+let test1 () : Tot unit = assert (forall h0 t. dlisthead_is_valid h0 (empty_list #t))
 
-let singletonlist (#t:eqtype) (e:ref (dlist t)) =
+val singletonlist: #t:eqtype -> e:ref (dlist t) ->
+  ST (dlisthead t)
+  (requires (fun _ -> True))
+  (ensures (fun h0 y h1 -> modifies (only e) h0 h1 /\ dlisthead_is_valid h1 y))
+let singletonlist #t e =
   e := { !e with blink = None; flink = None };
   { lhead = Some e ; ltail = Some e ; nodes = hide (Seq.create 1 (!e)) }
 
-let member_of (#t:eqtype) (h0:heap) (h:dlisthead t) (e:ref (dlist t)) =
+let member_of (#t:eqtype) (h0:heap) (h:dlisthead t) (e:ref (dlist t)) : GTot bool =
   Seq.mem (e@h0) (reveal h.nodes)
 
 type nonempty_dlisthead t = (h:dlisthead t{isSome h.lhead /\ isSome h.ltail})
 
-let (~.) (#t:Type) (a:t) : Tot (erased (seq t)) = hide (Seq.create 1 a)
-let (^+) (#t:Type) (a:t) (b:erased (seq t)) : Tot (erased (seq t)) = elift2 Seq.cons (hide a) b
+unfold let (~.) (#t:Type) (a:t) : Tot (erased (seq t)) = hide (Seq.create 1 a)
+unfold let (^+) (#t:Type) (a:t) (b:erased (seq t)) : Tot (erased (seq t)) = elift2 Seq.cons (hide a) b
 
-let dlisthead_make_valid_singleton (#t:eqtype) (h:nonempty_dlisthead t)
-  : ST (dlisthead t)
+val dlisthead_make_valid_singleton: #t:eqtype -> h:nonempty_dlisthead t ->
+  ST (dlisthead t)
     (requires (fun h0 ->
          isNone (h.lhead^@h0).flink /\ isNone (h.lhead^@h0).blink))
-    (ensures (fun h1 y h2 -> modifies_none h1 h2 /\ dlisthead_is_valid h2 y)) =
+    (ensures (fun h1 y h2 -> modifies_none h1 h2 /\ dlisthead_is_valid h2 y))
+let dlisthead_make_valid_singleton #t h =
   let Some e = h.lhead in
   { h with ltail = h.lhead ; nodes = ~. !e }
 
-let ghost_tail (#t:Type) (s:erased (seq t){Seq.length (reveal s) > 0}) : Tot (erased (seq t)) =
+unfold let ghost_tail (#t:Type) (s:erased (seq t){Seq.length (reveal s) > 0}) : Tot (erased (seq t)) =
   hide (Seq.tail (reveal s))
 
 val ghost_tail_properties :
@@ -116,10 +127,11 @@ let ghost_tail_properties #t s = ()
 
 #set-options "--z3rlimit 1 --detail_errors --z3rlimit_factor 20"
 
-let dlisthead_update_head (#t:eqtype) (h:nonempty_dlisthead t) (e:ref (dlist t))
-  : ST (dlisthead t)
-      (requires (fun h0 -> dlisthead_is_valid h0 h /\ ~(member_of h0 h e)))
-      (ensures (fun h1 y h2 -> modifies (e ^+^ (getSome h.lhead)) h1 h2 /\ dlisthead_is_valid h2 y)) =
+val dlisthead_update_head: #t:eqtype -> h:nonempty_dlisthead t -> e:ref (dlist t) ->
+  ST (dlisthead t)
+    (requires (fun h0 -> dlisthead_is_valid h0 h /\ ~(member_of h0 h e)))
+    (ensures (fun h1 y h2 -> modifies (e ^+^ (getSome h.lhead)) h1 h2 /\ dlisthead_is_valid h2 y))
+let dlisthead_update_head (#t:eqtype) (h:nonempty_dlisthead t) (e:ref (dlist t)) =
   let h1 = ST.get () in
   let Some n = h.lhead in
   e := { !e with blink = None; flink = Some n };
@@ -146,9 +158,11 @@ let dlisthead_update_head (#t:eqtype) (h:nonempty_dlisthead t) (e:ref (dlist t))
     y
   )
 
-let insertHeadList (#t:eqtype) (h:dlisthead t) (e:ref (dlist t)): ST (dlisthead t)
-   (requires (fun h0 -> dlisthead_is_valid h0 h /\ ~(member_of h0 h e)))
-   (ensures (fun _ y h2 -> dlisthead_is_valid h2 y)) =
+val insertHeadList: #t:eqtype -> h:dlisthead t -> e:ref (dlist t) ->
+  ST (dlisthead t)
+    (requires (fun h0 -> dlisthead_is_valid h0 h /\ ~(member_of h0 h e)))
+    (ensures (fun _ y h2 -> dlisthead_is_valid h2 y))
+let insertHeadList #t h e =
   if isNone h.lhead
   then (
     singletonlist e
